Add some comments/examples to the assignment operator

Hoare/Examples/Assign_example.lean
@@ -19,3 +19,27 @@ theorem foo_holds' : TripleHolds foo := by
   let foo_expr := [expr| X + 1]
   apply TripleHolds.assign' foo_stmt foo_expr "X" foo_com
 
+def foo' : Triple :=
+{(X + 1) == 2}
+X := X + 2
+{X == 2}
+
+-- Now we can prove that `X := X + 2` also changes `X` from 1 to 2.
+-- There's something funky happening here!
+-- (See Logic.lean)
+theorem foo'_holds : TripleHolds foo' := by
+  let foo_stmt := foo'.3
+  let foo_com := foo'.2
+  let foo_expr := [expr| X + 1]
+  apply TripleHolds.assign' foo_stmt foo_expr "X" foo_com
+
+
+#reduce [stmt| X == 1].subst "X" [expr| X + 1]
+
+-- This fails! There's another problem we have, namely that we're comparing syntactic equality of stmts, not their semantics.
+example : [stmt| X == 1].subst "X" [expr| X + 1] = [stmt| X == 2] := by
+  simp [Statement.subst, Expr.subst]
+
+-- Ideally, this should "just" work for this to be realtively useful.
+example : TripleHolds {X == 1} X := X + 1 {X == 2} := by
+   apply TripleHolds.assign -- I would hope this shold "just work"
